stage0/stdlib/Lean/Elab/App.c
@@ -454,6 +454,7 @@ LEAN_EXPORT lean_object* l___private_Lean_Elab_App_0__Lean_Elab_Term_findBinderN
 static lean_object* l_Lean_Elab_Term_initFn____x40_Lean_Elab_App___hyg_6491____lambda__1___closed__24;
 static lean_object* l_Std_Range_forIn_loop___at___private_Lean_Elab_App_0__Lean_Elab_Term_addLValArg___spec__1___closed__6;
 LEAN_EXPORT lean_object* l_Lean_Elab_Term_elabAppArgs___lambda__4(lean_object*, lean_object*, lean_object*, uint8_t, uint8_t, uint8_t, lean_object*, lean_object*, lean_object*, lean_object*, lean_object*, lean_object*, lean_object*, lean_object*, lean_object*, lean_object*, lean_object*);
+lean_object* l_Array_insertAt_x21___rarg(lean_object*, lean_object*, lean_object*);
 static lean_object* l___private_Lean_Elab_App_0__Lean_Elab_Term_elabAppLVals___closed__2;
 LEAN_EXPORT lean_object* l_panic___at___private_Lean_Elab_App_0__Lean_Elab_Term_mergeFailures___spec__1(lean_object*);
 LEAN_EXPORT lean_object* l_List_foldlM___at___private_Lean_Elab_App_0__Lean_Elab_Term_elabAppFnId___spec__1___lambda__1___boxed(lean_object**);
@@ -1213,7 +1214,6 @@ LEAN_EXPORT lean_object* l___private_Lean_MetavarContext_0__Lean_DependsOn_dep_v
 LEAN_EXPORT lean_object* l___private_Lean_Elab_App_0__Lean_Elab_Term_elabAppFn___lambda__2(lean_object*, lean_object*, lean_object*, lean_object*, lean_object*, uint8_t, uint8_t, uint8_t, lean_object*, lean_object*, lean_object*, lean_object*, lean_object*, lean_object*, lean_object*, lean_object*);
 LEAN_EXPORT lean_object* l_Lean_Elab_Term_ElabElim_finalize___lambda__2(lean_object*, lean_object*, lean_object*, lean_object*, lean_object*, lean_object*, lean_object*, lean_object*, lean_object*, lean_object*, lean_object*, lean_object*, lean_object*, lean_object*, lean_object*);
 lean_object* l_Lean_Expr_constName_x21(lean_object*);
-lean_object* l_Array_insertAt___rarg(lean_object*, lean_object*, lean_object*);
 LEAN_EXPORT lean_object* l___private_Lean_Elab_App_0__Lean_Elab_Term_throwLValError(lean_object*);
 static lean_object* l_Lean_Elab_Term_initFn____x40_Lean_Elab_App___hyg_6491____closed__1;
 static lean_object* l_Lean_Elab_Term_elabAppArgs___lambda__2___closed__2;
@@ -35365,7 +35365,7 @@ lean_inc(x_3);
 x_76 = lean_alloc_ctor(1, 1, 0);
 lean_ctor_set(x_76, 0, x_3);
 lean_inc(x_4);
-x_77 = l_Array_insertAt___rarg(x_4, x_35, x_76);
+x_77 = l_Array_insertAt_x21___rarg(x_4, x_35, x_76);
 lean_inc(x_5);
 x_78 = lean_alloc_ctor(0, 2, 0);
 lean_ctor_set(x_78, 0, x_77);
