stage0/stdlib/Lean/Meta/IndPredBelow.c
@@ -218,6 +218,7 @@ static lean_object* l_Lean_mkCasesOn___at_Lean_Meta_IndPredBelow_mkBelow___spec_
 LEAN_EXPORT lean_object* l_Lean_throwError___at_Lean_Meta_IndPredBelow_mkCtorType_mkBelowBinder___spec__1___rarg___boxed(lean_object*, lean_object*, lean_object*, lean_object*, lean_object*, lean_object*);
 LEAN_EXPORT lean_object* l_Lean_Expr_withAppAux___at_Lean_Meta_IndPredBelow_mkCtorType_mkMotiveBinder___spec__1___boxed(lean_object*, lean_object*, lean_object*, lean_object*, lean_object*, lean_object*, lean_object*, lean_object*, lean_object*, lean_object*, lean_object*, lean_object*, lean_object*, lean_object*, lean_object*);
 LEAN_EXPORT lean_object* l_Lean_Meta_IndPredBelow_mkCtorType_checkCount___lambda__2(lean_object*, lean_object*, lean_object*, lean_object*, lean_object*, lean_object*, lean_object*, lean_object*);
+lean_object* l_Array_insertAt_x21___rarg(lean_object*, lean_object*, lean_object*);
 LEAN_EXPORT lean_object* l_Array_mapIdxM_map___at_Lean_Meta_IndPredBelow_mkBelowDecl___spec__1(lean_object*, lean_object*, lean_object*, lean_object*, lean_object*, lean_object*, lean_object*, lean_object*, lean_object*, lean_object*, lean_object*);
 lean_object* l_Lean_MVarId_assign___at_Lean_Meta_getLevel___spec__1(lean_object*, lean_object*, lean_object*, lean_object*, lean_object*, lean_object*, lean_object*);
 static lean_object* l_Lean_Meta_IndPredBelow_mkBelowMatcher_convertToBelow___closed__6;
@@ -557,7 +558,6 @@ lean_object* l_Lean_Expr_constName_x21(lean_object*);
 static lean_object* l_Lean_Meta_IndPredBelow_proveBrecOn_closeGoal___closed__15;
 LEAN_EXPORT lean_object* l_Lean_Meta_IndPredBelow_proveBrecOn_closeGoal(lean_object*, lean_object*, lean_object*, lean_object*, lean_object*, lean_object*, lean_object*);
 LEAN_EXPORT lean_object* l_Lean_Meta_transform___at_Lean_Meta_IndPredBelow_mkCtorType_checkCount___spec__1___boxed(lean_object*, lean_object*, lean_object*, lean_object*, lean_object*, lean_object*, lean_object*, lean_object*, lean_object*, lean_object*);
-lean_object* l_Array_insertAt___rarg(lean_object*, lean_object*, lean_object*);
 lean_object* l_Array_indexOfAux___at___private_Lean_Meta_FunInfo_0__Lean_Meta_collectDeps_visit___spec__1(lean_object*, lean_object*, lean_object*);
 static lean_object* l_Array_mapIdxM_map___at_Lean_Meta_IndPredBelow_mkBelowMatcher___spec__3___lambda__1___closed__4;
 LEAN_EXPORT lean_object* l_Array_mapMUnsafe_map___at_Lean_Meta_IndPredBelow_mkCtorType_replaceTempVars___spec__3___boxed(lean_object*, lean_object*, lean_object*, lean_object*);
@@ -767,7 +767,7 @@ LEAN_EXPORT lean_object* l_Array_foldrMUnsafe_fold___at_Lean_Meta_IndPredBelow_m
 _start:
 {
 lean_object* x_10; uint8_t x_11; uint8_t x_12; uint8_t x_13; lean_object* x_14; 
-x_10 = l_Array_insertAt___rarg(x_1, x_2, x_4);
+x_10 = l_Array_insertAt_x21___rarg(x_1, x_2, x_4);
 x_11 = 0;
 x_12 = 1;
 x_13 = 1;
