stage0/stdlib/Lean/Meta/UnificationHint.c
@@ -137,6 +137,7 @@ lean_object* l_Lean_ScopedEnvExtension_addLocalEntry___rarg(lean_object*, lean_o
 LEAN_EXPORT lean_object* l_Std_PersistentHashMap_insertAux_traverse___at_Lean_Meta_UnificationHints_add___spec__7(size_t, lean_object*, lean_object*, lean_object*, lean_object*, lean_object*);
 lean_object* lean_nat_sub(lean_object*, lean_object*);
 LEAN_EXPORT lean_object* l_Array_forInUnsafe_loop___at_Lean_Meta_tryUnificationHints___spec__1(lean_object*, lean_object*, lean_object*, lean_object*, size_t, size_t, lean_object*, lean_object*, lean_object*, lean_object*, lean_object*, lean_object*);
+lean_object* l_Array_insertAt_x21___rarg(lean_object*, lean_object*, lean_object*);
 lean_object* l___private_Lean_Meta_DiscrTree_0__Lean_Meta_DiscrTree_createNodes___rarg(lean_object*, lean_object*, lean_object*);
 LEAN_EXPORT lean_object* l_Std_PersistentHashMap_insertAtCollisionNodeAux___at_Lean_Meta_UnificationHints_add___spec__8(lean_object*, lean_object*, lean_object*, lean_object*);
 LEAN_EXPORT lean_object* l_Std_PersistentHashMap_foldlM___at_Lean_Meta_instToFormatUnificationHints___spec__6(lean_object*, lean_object*, lean_object*);
@@ -313,7 +314,6 @@ LEAN_EXPORT lean_object* l_Lean_Meta_tryUnificationHints___lambda__1___boxed(lea
 lean_object* l_Lean_Meta_setPostponed(lean_object*, lean_object*, lean_object*, lean_object*, lean_object*, lean_object*);
 static lean_object* l_Lean_ScopedEnvExtension_add___at_Lean_Meta_addUnificationHint___spec__1___closed__5;
 lean_object* l_Lean_Meta_processPostponed(uint8_t, uint8_t, lean_object*, lean_object*, lean_object*, lean_object*, lean_object*);
-lean_object* l_Array_insertAt___rarg(lean_object*, lean_object*, lean_object*);
 LEAN_EXPORT lean_object* l_Array_forInUnsafe_loop___at_Lean_Meta_tryUnificationHints_tryCandidate___spec__3___boxed(lean_object*, lean_object*, lean_object*, lean_object*, lean_object*, lean_object*, lean_object*, lean_object*, lean_object*, lean_object*, lean_object*);
 static lean_object* l_Lean_Meta_DiscrTree_Trie_format___at_Lean_Meta_instToFormatUnificationHints___spec__2___closed__2;
 static lean_object* l_Lean_Meta_DiscrTree_insertCore___at_Lean_Meta_UnificationHints_add___spec__1___closed__6;
@@ -1903,7 +1903,7 @@ lean_ctor_set(x_42, 0, x_4);
 lean_ctor_set(x_42, 1, x_41);
 x_43 = lean_nat_add(x_8, x_39);
 lean_dec(x_8);
-x_44 = l_Array_insertAt___rarg(x_6, x_43, x_42);
+x_44 = l_Array_insertAt_x21___rarg(x_6, x_43, x_42);
 lean_dec(x_43);
 return x_44;
 }
@@ -2094,7 +2094,7 @@ lean_dec(x_65);
 x_67 = lean_alloc_ctor(0, 2, 0);
 lean_ctor_set(x_67, 0, x_4);
 lean_ctor_set(x_67, 1, x_66);
-x_68 = l_Array_insertAt___rarg(x_6, x_9, x_67);
+x_68 = l_Array_insertAt_x21___rarg(x_6, x_9, x_67);
 return x_68;
 }
 }
