stage0/stdlib/Lean/Parser/Extension.c
@@ -227,7 +227,7 @@ static lean_object* l_Lean_Parser_initFn____x40_Lean_Parser_Extension___hyg_5991
 static lean_object* l_Lean_Parser_initFn____x40_Lean_Parser_Extension___hyg_4136____closed__6;
 static lean_object* l_Lean_Parser_initFn____x40_Lean_Parser_Extension___hyg_84____closed__6;
 uint8_t lean_nat_dec_eq(lean_object*, lean_object*);
-uint8_t l___private_Lean_Attributes_0__Lean_beqAttributeKind____x40_Lean_Attributes___hyg_187_(uint8_t, uint8_t);
+uint8_t l___private_Lean_Attributes_0__Lean_beqAttributeKind____x40_Lean_Attributes___hyg_182_(uint8_t, uint8_t);
 static lean_object* l_Lean_Parser_initFn____x40_Lean_Parser_Extension___hyg_3693____closed__6;
 LEAN_EXPORT lean_object* l_Lean_Parser_getBinaryAlias___rarg___boxed(lean_object*, lean_object*, lean_object*);
 static lean_object* l___private_Lean_Parser_Extension_0__Lean_Parser_updateBuiltinTokens___closed__2;
@@ -11154,7 +11154,7 @@ x_11 = lean_ctor_get(x_9, 1);
 lean_inc(x_11);
 lean_dec(x_9);
 x_12 = 0;
-x_13 = l___private_Lean_Attributes_0__Lean_beqAttributeKind____x40_Lean_Attributes___hyg_187_(x_5, x_12);
+x_13 = l___private_Lean_Attributes_0__Lean_beqAttributeKind____x40_Lean_Attributes___hyg_182_(x_5, x_12);
 if (x_13 == 0)
 {
 lean_object* x_14; lean_object* x_15; lean_object* x_16; lean_object* x_17; lean_object* x_18; lean_object* x_19; uint8_t x_20; 
